iris/SpecFetchaddr.v
@@ -132,7 +132,7 @@ Definition wp_fetchaddr_sconf_body `{!riscvGS Σ, !xv6G Σ, !bioslotG Σ, !fdslo
        handed. *)
     ∀ (mf : regfile) (P' : uptd),
       ⌜callee_saved m mf⌝ -∗
-      ⌜uptd_ext (pv_upt (us_V U)) P'⌝ -∗
+      ⌜uptd_ext_sz (pv_sz (us_V U)) (pv_upt (us_V U)) P'⌝ -∗
       sie_cap_gpr KT1 mf av b p -∗
       cpu_own 0%nat eb p b lks -∗
       pc_is ret_tgt -∗
